Обозначим \(\sigma = \varepsilon^2\) и сделаем следующие замены:
\begin{equation}
    \tau = t\varepsilon^2, u = \varepsilon w, 
    \Hln (u, t) = \Fln (w, \tau, \varepsilon).
\end{equation}

\begin{equation}\begin{aligned}\label{F1FirstEquationParticular}
j\varepsilon wa(x) \Fln (w,\tau)&=  \\
   =&-\Q{\lambda+\allExecutionFullIntensity{n}{k}}\seqStandart{F^{(1)}}{n}(w,\tau)+\\
    &+j \varepsilon \En \pdv{\seqStandart{F^{(1)}}{n}(w,\tau)}{w} - \\
    &-x \En \seqStandart{F^{(1)}}{n}(w,\tau) + \\
    &+\overline{\En} \lambda e^{j\varepsilon w} \seqStandart{F^{(1)}}{n}(w,\tau)+\\
    &+r_1 \Q{\allExecutionRelativeIntensity{n}{k}} \seqStandart{F^{(1)}}{n}(w,\tau) + \\
    &+\lambda\sum_{k=0}^{M-1}q_k \seqMinus{F^{(1)}}{n}{k}(w,\tau) + \\
    &-j \varepsilon  e^{-j\varepsilon w} \sum_{k=0}^{M-1}q_k \pdv{\seqMinus{F^{(1)}}{n}{k}(w,\tau)}{w} + \\
    &+x  e^{-j\varepsilon w} \sum_{k=0}^{M-1}q_k \seqMinus{F^{(1)}}{n}{k}(w,\tau) + \\
    &+\En r_0 \sum_{f=0}^{M-1} \mu_f (n_f + 1) \seqPlus{F^{(1)}}{n}{f}(w,\tau) + \\
    &+\En r_2 e^{j\varepsilon w} \sum_{f=0}^{M-1} \mu_f (n_f + 1) \seqPlus{F^{(1)}}{n}{f}(w,\tau) + \\
    &+r_1 \feedbackSum{f}{k}
        q_k \mu_f (n_f+1) \seqMinusPlus{F^{(1)}}{n}{k}{f}(w,\tau),
\end{aligned}\end{equation}

\begin{equation}\begin{aligned}\label{F1SecondEquationParticular}
\nJ \Bigg[ \pdv{\Fln(w,\tau)}{\tau} & + j\varepsilon wa(x) \Hln (w,\tau) \Bigg] = \\
=(e^{j\varepsilon w} - 1)
\Bigg\{
    &\lambda \nI \seqStandart{F^{(1)}}{n}(w,\tau)+\\
    &+j\varepsilon e^{-j\varepsilon w} \nG\pdv{\seqStandart{F^{(1)}}{n}(w,\tau)}{w} + \\
    &-x e^{-j\varepsilon w} \nG \seqStandart{F^{(1)}}{n}(w,\tau) + \\
    &+r_2\sum_{f=0}^{M-1} \mu_f \nJ n_f \seqStandart{F^{(1)}}{n}(w,\tau)
\Bigg\}
.
\end{aligned}\end{equation}


