Рассмотрим \eqref{FFirstEquationParticular}, введя обозначение:
\[\lim_{\varepsilon \to 0} \Fn(w, \tau, \varepsilon) =
    \Fn(w, \tau),\]

\begin{equation}\begin{aligned}
\label{FLimitEquationParticular}
0=
    &-\Q{\lambda+\allExecutionFullIntensity{n}{k}}\seqStandart{F}{n}(w,\tau)+\\
    &+j \En \pdv{\seqStandart{F}{n}(w,\tau)}{w}(i,\tau) + \\
    &+\overline{\En} \lambda \seqStandart{F}{n}(w,\tau)+\\
    &+r_1 \Q{\allExecutionRelativeIntensity{n}{k}} \seqStandart{F}{n}(w,\tau) + \\
    &+\lambda\sum_{k=1}^{M}q_k \seqMinus{F}{n}{k}(w,\tau) + \\
    &-j\sum_{k=1}^{M}q_k \pdv{\seqMinus{F}{n}{k}(w,\tau)}{w} + \\
    &+\En r_0 \sum_{f=1}^{M} \mu_f (n_f + 1) \seqPlus{F}{n}{f}(w,\tau) + \\
    &+\En r_2 \sum_{f=1}^{M} \mu_f (n_f + 1) \seqPlus{F}{n}{f}(w,\tau) + \\
    &+r_1 \feedbackSum{f}{k}
        q_k \mu_f (n_f+1) \seqMinusPlus{F}{n}{k}{f}(w,\tau).
\end{aligned}\end{equation}

Будем искать решение в виде \(\Fn = \Rn e^{jwx(\tau)}\):
\begin{equation} \label{RSumEqualsToOne}
    1 = \sum_{\bold{n}}^{\Jt}\Rn,
\end{equation}
\begin{equation}\begin{aligned} \label{RFirstEverParticular}
0=
    &-\Q{\lambda+\allExecutionFullIntensity{n}{k}}\seqStandart{R}{n}+\\
    &-\En x(\tau) \seqStandart{R}{n} + \\
    &+\overline{\En} \lambda \seqStandart{R}{n} +\\
    &+r_1 \Q{\allExecutionRelativeIntensity{n}{k}} \seqStandart{R}{n} + \\
    &+\lambda\sum_{k=1}^{M}q_k \seqMinus{R}{n}{k} + \\
    &+\sum_{k=1}^{M}q_k \seqMinus{R}{n}{k} + \\
    &+\En r_0 \sum_{f=1}^{M} \mu_f (n_f + 1) \seqPlus{R}{n}{f} + \\
    &+\En r_2 \sum_{f=1}^{M} \mu_f (n_f + 1) \seqPlus{R}{n}{f} + \\
    &+r_1 \feedbackSum{f}{k}
        q_k \mu_f (n_f+1) \seqMinusPlus{R}{n}{k}{f}.
\end{aligned}\end{equation}

В \eqref{RFirstEverParticular} приведём подобные:
\begin{equation}\begin{aligned} \label{REquationParticular}
0=
    &-\Q{\En \T{\lxt}+\allExecutionFullIntensity{n}{k}}\seqStandart{R}{n}+\\
    &+r_1 \Q{\allExecutionRelativeIntensity{n}{k}} \seqStandart{R}{n} + \\
    &+\T{\lxt}\sum_{k=1}^{M}q_k \seqMinus{R}{n}{k} + \\
    &+\En (1 - r_1) \sum_{f=1}^{M} \mu_f (n_f + 1) \seqPlus{R}{n}{f} + \\
    &+r_1 \feedbackSum{f}{k}
        q_k \mu_f (n_f+1) \seqMinusPlus{R}{n}{k}{f}.
\end{aligned}\end{equation}


