Обозначим:
\begin{gather*}
	\boldsymbol{H}(u,t) = \bigg[H_{\tilde{1}}(u,t), H_{\tilde{2}}(u,t), ... H_{\tilde{|\mathbb{J}|} }(u,t)\bigg] ,\\
	\boldsymbol{C} = ||C_{\tilde{n},\tilde{m}}||,
	\text{ }\text{ }\text{ }\text{ }\text{ }
	\boldsymbol{B} = ||B_{\tilde{n},\tilde{m}}||,
	\text{ }\text{ }\text{ }\text{ }\boldsymbol{D} = \bigg|\bigg|\delta_{n,m}
	\sum_{\nu = 1}^{|\mathbb{J}|}\bigg(C_{\tilde{\nu},\tilde{n}} + B_{\tilde{\nu},\tilde{n}} \bigg)\bigg|\bigg|, \\
	\boldsymbol{K} = ||K_{\tilde{n},\tilde{m}}||,
	\text{ }\text{ }\text{ }\text{ }\boldsymbol{I} = \bigg|\bigg|\delta_{n,m}
	\sum_{\nu = 1}^{|\mathbb{J}|}K_{\tilde{\nu},\tilde{n}}\bigg|\bigg|.
\end{gather*}
И получим:
\begin{equation}\label{pervoe_uravnenie_partial}
    \pdv{\boldsymbol{H}(u,t)}{t} =
    \boldsymbol{H}(u,t)\bigg[\boldsymbol{C} + e^{ju}\boldsymbol{B} - \boldsymbol{D}\bigg]
    -j\eta\pdv{\boldsymbol{H}(u,t)}{u}\bigg[e^{-ju}\boldsymbol{K} - \boldsymbol{I}\bigg].
\end{equation}
